Stating the measure.

theories/common.v
@@ -456,6 +456,15 @@ Proof.
   - move => ? ? A. inversion A.
 Qed.
 
+Lemma maxn_nat_max : forall n m,
+  maxn n m = Nat.max n m.
+Proof.
+  move=> n m. rewrite /maxn. case E: (n < m).
+  - rewrite Max.max_r => //. by lias.
+  - rewrite -> Max.max_l => //. have: (~ n < m)%coq_nat; last by lias.
+    move: E => /negP E I. apply: E. by lias.
+Qed.
+
 
 (** * An equivalent to [List.Forall], but in [Type] instead of [Prop]. **)
 
@@ -469,7 +478,13 @@ Inductive Forall (A : Type) (P : A -> Type) : seq A -> Type :=
 Fixpoint max A l (F : Forall (fun (_ : A) => nat) l) : nat :=
   match F with
   | Forall_nil => 0
-  | Forall_cons _ _ n F => Nat.max n (max F)
+  | Forall_cons _ _ n F => maxn n (max F)
+  end.
+
+Fixpoint sum A l (F : Forall (fun (_ : A) => nat) l) : nat :=
+  match F with
+  | Forall_nil => 0
+  | Forall_cons _ _ n F => n + (sum F)
   end.
 
 Fixpoint map A P Q (f : forall a, P a -> Q a) (l : seq A) (F : Forall P l) : Forall Q l :=
@@ -519,33 +534,33 @@ Proof.
   move=> > F. apply List.Forall_forall. by apply: Forall_forall F.
 Qed.
 
-Definition List_Forall_Forall : forall A (P : A -> Prop) l,
+Lemma List_Forall_Forall : forall A (P : A -> Prop) l,
   List.Forall P l ->
   Forall P l.
 Proof.
   move=> > F. apply: forall_Forall. by apply List.Forall_forall.
 Defined.
 
-Definition Forall_cat A (P : A -> Prop) (l1 l2 : list A) (F1 : Forall P l1) (F2 : Forall P l2)
+Lemma Forall_cat A (P : A -> Prop) (l1 l2 : list A) (F1 : Forall P l1) (F2 : Forall P l2)
   : Forall P (l1 ++ l2).
 Proof.
   induction F1 => //. by apply: Forall_cons.
 Defined.
 
-Definition Forall_catrev A (P : A -> Prop) : forall (l1 l2 : list A),
+Lemma Forall_catrev A (P : A -> Prop) : forall (l1 l2 : list A),
   Forall P l1 -> Forall P l2 -> Forall P (rev l1 ++ l2).
 Proof.
   move=> l1 + F1. induction F1 => // l2 F2.
   rewrite rev_cons -cats1 -catA. apply: IHF1. by apply: Forall_cons.
 Defined.
 
-Definition Forall_rev A (P : A -> Prop) (l : list A) (F : Forall P l) : Forall P (rev l).
+Lemma Forall_rev A (P : A -> Prop) (l : list A) (F : Forall P l) : Forall P (rev l).
 Proof.
   rewrite -(cats0 (rev l)). apply: Forall_catrev => //. by apply: Forall_nil.
 Defined.
 
 (* FIXME: There are too many opaque things there: I’m afraid that this is not provable.
-Definition Forall_catrevE : forall A (P : A -> Prop) l1 l2 (F1 : Forall P l1) (F2 : Forall P l2),
+Lemma Forall_catrevE : forall A (P : A -> Prop) l1 l2 (F1 : Forall P l1) (F2 : Forall P l2),
   Forall_catrev F1 F2 = Forall_cat (Forall_rev F1) F2.
 Proof.
   move=> A P l1 + F1. induction F1 => l2 F2.
@@ -553,7 +568,23 @@ Proof.
 Qed.
 *)
 
-Definition Forall_forall_eq_dec : forall A l1 l2,
+Lemma max_to_list A (l : seq A) (F : Forall _ l) :
+  max F = foldr maxn 0 (to_list F).
+Proof.
+  elim F.
+  - done.
+  - move=> a l' p f E /=. by rewrite E.
+Qed.
+
+Lemma sum_to_list A (l : seq A) (F : Forall _ l) :
+  sum F = foldr addn 0 (to_list F).
+Proof.
+  elim F.
+  - done.
+  - move=> a l' p f E /=. by rewrite E.
+Qed.
+
+Lemma Forall_forall_eq_dec : forall A l1 l2,
   Forall (fun x : A => forall y, {x = y} + {x <> y}) l1 ->
   {l1 = l2} + {l1 <> l2}.
 Proof.
